proof/ConRon/Refine2/Inductives/Prims.lean
@@ -272,7 +272,7 @@ open Lockstep in
     (hfe : IFEnvRelI rf lf) :
     LS pers (fun a b => b = id a) (arena.checker_base.consts_resolve_f_fast pers vis st rf e) lst
       (constsResolveFFast (lf.restrictTo (absU vis)) (absEIdx e)) :=
-  LS.ofSim₀ fun _ h => consts_resolve_f_fast_refines hrel hinv hfe.rel hfe.inv h
+  ConRon.Refine2.consts_resolve_f_fast_ls hrel hinv hfe
 
 
 open Lockstep in
@@ -284,7 +284,7 @@ open Lockstep in
     (hinv : AStateInv pers st) :
     LSR pers (fun a b => b = id a) (arena.checker_base.all_level_params_defined pers st lps e) st lst
                    (allLevelParamsDefined (absNIdxL lps) (absEIdx e)) :=
-  LSR.ofSimRE hrel hinv fun _ h => all_level_params_defined_refines hrel hinv h
+  ConRon.Refine2.all_level_params_defined_ls hrel hinv
 
 
 open Lockstep in
